\section{Backup}
\begin{frame}
	\frametitle{Why does $\gamma_\mu\Psi^\mu$ transform like a dirac spinor.}
	The Dirac part of the vector-spinor spinor transform like
	\begin{equation*}
		\Psi^{\mu'} = \Lambda^\mu_{\ \nu}M(\Lambda) \Psi^\nu
	\end{equation*}
	Also we need the property
	\begin{equation*}
		M(\Lambda)\gamma_\mu M^{-1}(\Lambda) = \Lambda^{\nu}_{\ \mu} \gamma_{\nu}
	\end{equation*}
	To show 
	\begin{align*}
		(\gamma_\mu\Psi^\mu)' = \gamma_\mu  \Lambda^\mu_{\ \nu}M(\Lambda) \Psi^\nu
		= M(\Lambda)\gamma_\mu M^{-1}(\Lambda)M(\Lambda) \Psi^\nu
		= M(\Lambda) \gamma_\nu\Psi^\nu
	\end{align*}
\end{frame}
